1) The proof of filter (r3969) was correct, but not strong enough at all cases. Filter proved that if a function does not use the variable defined in a pure cmd of the function, then we can remove the cmd. Here is a case,
mem2reg calls DIE after LAS to remove the load, because all uses of the variable
 lid defined by the load were already substed. But, to conclude that no one
uses lid, we need to show that the substituting value v (in this case,
which is the value stored alive to the load) does not contain lid. If
the store is in a reachable block, this is true, otherwise, v can
contain lid. So, in term of the 3969's DIE, the lid is not removable.

Actually, it is fine to remove a variable if the variable is not used
only when the variable is defined in a reachable block. If the variable
to remove is in an unreachable block, other unreachable blocks can still
use it. In the case, it is still safe to remove, because unreachable
blocks have no effects. So, we strengthened die.v (simulation) in this way. 
LAS's output program holds the new condition.

The alternative is that mem2reg should check the condition explicitly.
But, this introduces compile-time cost. 

die_wfS.v is broken. We need to strenthen filter.v to meet the same
condition.

2) Note that this statement in r3969 was already an extension of 
Vminus/removal.v that does not require that there exists a cmd in the
function that defines the variable. Vminus/removal.v is not sufficient to prove
 that removing a cmd whose id equals to the id of a dead store is safe.



git-svn-id: https://webdav.seas.upenn.edu/svn/sol/vol@3970 eef5ea85-cc2e-0410-bd84-0fae1f012da8

src3.0/Transforms/die.v
@@ -13,6 +13,8 @@ Require Import palloca_props.
 Require Import top_sim.
 Require Import trans_tactic.
 
+(**********************************************)
+
 Definition pure_cmd (instr:insn) : Prop :=
 match instr with
 | insn_cmd c =>
@@ -33,7 +35,7 @@ Record DIInfo := mkDIInfo {
   DI_pure : forall instr,
                lookupInsnViaIDFromFdef DI_f DI_id = Some instr ->
                pure_cmd instr;
-  DI_unused : used_in_fdef DI_id DI_f = false
+  DI_unused : runused_in_fdef DI_id DI_f
 }.
 
 Definition fdef_simulation (diinfo: DIInfo) f1 f2 : Prop :=
@@ -171,10 +173,9 @@ Qed.
 Lemma getIncomingValuesForBlockFromPHINodes_rsim : forall los nts B1 B2 gl F
   lc1' dinfo lc2' ps
   (Hnuse: DI_f dinfo <> F \/ ~ In (DI_id dinfo) (getPhiNodesIDs ps))
-  (Hnuse': DI_f dinfo <> F \/
-           fold_left
-             (fun (re : bool) (p : phinode) => re || used_in_phi (DI_id dinfo) p)
-           ps false = false)
+  (Hnuse': forall pn v (Hin: In pn ps)
+             (Hget: getValueViaBlockFromPHINode pn B1 = Some v),
+             conditional_used_in_value (DI_f dinfo) F (DI_id dinfo) v)
   (l3 l0:list (id * GVsT DGVs))
   (HeqR0 : Opsem.getIncomingValuesForBlockFromPHINodes (los,nts) ps B1 gl lc1' =
            ret l3)
@@ -198,43 +199,28 @@ Proof.
       assert (DI_f dinfo <> F \/ ~ In (DI_id dinfo) (getPhiNodesIDs ps)) as J3.
         clear - Hnuse.
         destruct Hnuse as [Hnuse | Hnuse]; auto.
-      assert (DI_f dinfo <> F \/
-              fold_left
-                (fun (re : bool) (p : phinode) =>
-                  re || used_in_phi (DI_id dinfo) p)
-                 ps false = false) as J4.
-        clear - Hnuse'.
-        destruct Hnuse' as [Hnuse' | Hnuse']; auto.
-        right.
-        assert (J:=Hnuse').
-        apply fold_left_eq in J.
-          rewrite J in Hnuse'. auto.
-          intros. apply orb_false_iff in H. destruct H; auto.
-      apply IHps; auto.
+      apply IHps; eauto 2.
+        intros. eapply Hnuse' in Hget; eauto.
     erewrite RemoveSim.block_simulation__getValueViaBlockFromValuels in HeqR3; 
       eauto.
     erewrite simulation__getOperandValue in HeqR0; eauto.
       repeat uniq_result. 
       apply reg_simulation_update; auto.
 
-      destruct B2. simpl in HeqR3.
-      assert (DI_f dinfo <> F \/ used_in_list_value_l (DI_id dinfo) l0 = false)
-        as J3.
-        clear - Hnuse'.
-        destruct Hnuse' as [Hnuse' | Hnuse']; auto.
-        right.
-        apply fold_left_eq in Hnuse'; auto.
-          intros. apply orb_false_iff in H. destruct H; auto.
-      eapply conditional_used_in_getValueViaLabelFromValuels; eauto 1.
+      assert (getValueViaBlockFromPHINode (insn_phi i0 typ5 l0) B1 = Some v0) 
+        as Hget'.
+        simpl. destruct B1, B2.
+        apply RemoveSim.block_simulation_inv in Hbsim2.
+        destruct Hbsim2; subst. simpl. auto.
+      eapply Hnuse'; eauto.
 Qed.
 
 Lemma switchToNewBasicBlock_rsim : forall los nts l1 l2 ps cs1 cs2 tmn1 tmn2 B1 
-  B2 gl lc1 lc2 F dinfo lc1' lc2' 
-  (Hnuse': DI_f dinfo <> F \/
-           fold_left
-             (fun (re : bool) (p : phinode) => re || used_in_phi (DI_id dinfo) p)
-           ps false = false)
-  (Huniq: uniqFdef F)
+  B2 gl lc1 lc2 F dinfo lc1' lc2' Ps S
+  (Hreach: isReachableFromEntry F B1) 
+  (HBinF1: blockInFdefB B1 F = true)
+  (HBinF1': blockInFdefB (block_intro l2 ps cs2 tmn2) F = true)
+  (Huniq: uniqFdef F) (HwfF: wf_fdef S (module_intro los nts Ps) F)
   (HBinF: blockInFdefB (block_intro l1 ps cs1 tmn1) F = true)
   (H23 : @Opsem.switchToNewBasicBlock DGVs (los,nts)
           (block_intro l1 ps cs1 tmn1) B1 gl lc1' =
@@ -248,9 +234,12 @@ Proof.
   intros.
   unfold Opsem.switchToNewBasicBlock in *. simpl in *.
   inv_mbind'. symmetry_ctx.
-  eapply getIncomingValuesForBlockFromPHINodes_rsim; eauto.
+  eapply getIncomingValuesForBlockFromPHINodes_rsim; eauto 1.
     destruct (fdef_dec (DI_f dinfo) F); subst; auto.
       right. eapply dont_remove_phinodes; eauto.
+    intros. destruct dinfo. simpl in *.
+    eapply conditional_runused_in_fdef__used_in_getValueViaBlockFromPHINode; 
+      eauto.
 Qed.
 
 Definition list_value_doesnt_use_did dinfo F idxs :=
@@ -416,9 +405,9 @@ match goal with
              |},
   Hwfpp : OpsemPP.wf_State
             {|
-            OpsemAux.CurSystem := _;
+            OpsemAux.CurSystem := ?S;
             OpsemAux.CurTargetData := ?TD;
-            OpsemAux.CurProducts := _;
+            OpsemAux.CurProducts := ?Ps;
             OpsemAux.Globals := _;
             OpsemAux.FunTable := _
              |} _,
@@ -442,59 +431,13 @@ match goal with
   destruct Hecsim as
       [Hfsim2 [Heq1 [Halsim2 [Hbsim2
         [Heq3 [Heq4 [Hlcsim2 Hcssim2]]]]]]]; subst;
-  assert (Heq3':=Heq3); destruct Heq3' as [l3 [ps1 [cs11 Heq3']]]; subst
-end.
-
-Ltac destruct_ctx_return :=
-match goal with
-| Hwfcfg : OpsemPP.wf_Config
-            {|
-            OpsemAux.CurSystem := _;
-            OpsemAux.CurTargetData := ?TD;
-            OpsemAux.CurProducts := _;
-            OpsemAux.Globals := _;
-            OpsemAux.FunTable := _
-             |},
-  Hwfpp : OpsemPP.wf_State
-            {|
-            OpsemAux.CurSystem := _;
-            OpsemAux.CurTargetData := ?TD;
-            OpsemAux.CurProducts := _;
-            OpsemAux.Globals := _;
-            OpsemAux.FunTable := _
-             |} _,
-  Hsim : State_simulation _ _ _ ?Cfg2 ?St2 ,
-  Hop2 : Opsem.sInsn _ _ _ _ |- _ =>
-  destruct TD as [los nts];
-  destruct Hwfcfg as [_ [Hwfg [HwfSystem HmInS]]];
-  destruct Hwfpp as
-    [_ [
-     [Hreach1 [HBinF1 [HFinPs1 _]]]
-     [
-       [
-         [Hreach2 [HBinF2 [HFinPs2 _]]]
-         _
-       ]
-       HwfCall'
-     ]]
-    ]; subst;
-  destruct Cfg2 as [S2 TD2 Ps2 gl2 fs2];
-  destruct St2 as [ECs2 M2];
-  simpl in Hsim;
-  destruct Hsim as [EQ1 [Hpsim [Hstksim [EQ2 [EQ3 Hmsim]]]]]; subst;
-  destruct ECs2 as [|[F2 B2 cs2 tmn2 lc2 als2] ECs2]; tinv Hstksim;
-  destruct Hstksim as [Hecsim Hstksim];
-  destruct ECs2 as [|[F3 B3 cs3 tmn3 lc3 als3] ECs2]; tinv Hstksim;
-  destruct Hstksim as [Hecsim' Hstksim];
-  unfold EC_simulation in Hecsim;
-  destruct Hecsim as
-      [Hfsim2 [Heq1 [Halsim2 [Hbsim2
-        [Heq3 [Heq4 [Hlcsim2 Hcssim2]]]]]]]; subst;
-  destruct Hecsim' as
-      [Hfsim2' [Heq1' [Halsim2' [Hbsim2'
-        [Heq3' [Heq4' [Hlcsim2' Hcssim2']]]]]]]; subst;
-  apply RemoveSim.cmds_simulation_nil_inv in Hcssim2; subst;
-  wfCall_inv
+  assert (Heq3':=Heq3); destruct Heq3' as [l3 [ps1 [cs11 Heq3']]]; subst;
+  match goal with 
+  | _: block_simulation _ ?F _ _ |- _ =>
+    assert (HwfF: wf_fdef S (module_intro los nts Ps) F) by
+      eauto 2 using wf_system__wf_fdef;
+    assert (HuniqF: uniqFdef F) by eauto 2 using wf_system__uniqFdef
+  end
 end.
 
 Definition removable_State (dinfo: DIInfo) (St:@Opsem.State DGVs) : Prop :=
@@ -566,25 +509,6 @@ Proof.
     ).
 Qed.
 
-Ltac value_doesnt_use_did_tac :=
-match goal with
-| |- value_doesnt_use_did ?diinfo _ _ =>
-  try solve [
-    eapply conditional_used_in_fdef__used_in_tmn_value; 
-      destruct diinfo; eauto; simpl; auto |
-    eapply conditional_used_in_fdef__used_in_cmd_value; 
-      destruct diinfo; eauto 1 using in_middle; simpl; auto
-  ]
-| |- DI_f ?diinfo <> _ \/
-     fold_left
-       (fun (re : bool) (p : phinode) => re || used_in_phi (DI_id ?diinfo) p)
-       _ false = false =>
-  eapply conditional_used_in_fdef__used_in_phis; destruct diinfo; eauto
-| |- list_value_doesnt_use_did ?diinfo _ _ =>
-    eapply conditional_used_in_fdef__used_in_list_value; 
-      destruct diinfo; eauto using in_middle; simpl; auto
-end.  
-
 Lemma simulation__values2GVs : forall lc lc2 los nts gl F idxs 
   dinfo (Hprop: list_value_doesnt_use_did dinfo F idxs),
   reg_simulation dinfo F lc lc2 ->
@@ -606,6 +530,20 @@ Proof.
     erewrite simulation__getOperandValue; eauto.
     erewrite IHidxs; eauto.
 Qed.
+
+Ltac value_doesnt_use_did_tac :=
+match goal with
+| |- value_doesnt_use_did ?diinfo _ _ =>
+  try solve [
+    eapply conditional_runused_in_fdef__used_in_tmn_value; 
+      destruct diinfo; eauto; simpl; auto |
+    eapply conditional_runused_in_fdef__used_in_cmd_value; 
+      destruct diinfo; eauto 1 using in_middle; simpl; auto
+  ]
+| |- list_value_doesnt_use_did ?diinfo _ _ =>
+    eapply conditional_runused_in_fdef__used_in_list_value; 
+      destruct diinfo; eauto 1 using in_middle; simpl; auto
+end.  
 
 Ltac simulation__getOperandValue_tac :=
 match goal with
@@ -701,6 +639,64 @@ match goal with
   ]
 end.
 
+Ltac destruct_ctx_return :=
+match goal with
+| Hwfcfg : OpsemPP.wf_Config
+            {|
+            OpsemAux.CurSystem := _;
+            OpsemAux.CurTargetData := ?TD;
+            OpsemAux.CurProducts := _;
+            OpsemAux.Globals := _;
+            OpsemAux.FunTable := _
+             |},
+  Hwfpp : OpsemPP.wf_State
+            {|
+            OpsemAux.CurSystem := ?S;
+            OpsemAux.CurTargetData := ?TD;
+            OpsemAux.CurProducts := ?Ps;
+            OpsemAux.Globals := _;
+            OpsemAux.FunTable := _
+             |} _,
+  Hsim : State_simulation _ _ _ ?Cfg2 ?St2 ,
+  Hop2 : Opsem.sInsn _ _ _ _ |- _ =>
+  destruct TD as [los nts];
+  destruct Hwfcfg as [_ [Hwfg [HwfSystem HmInS]]];
+  destruct Hwfpp as
+    [_ [
+     [Hreach1 [HBinF1 [HFinPs1 _]]]
+     [
+       [
+         [Hreach2 [HBinF2 [HFinPs2 _]]]
+         _
+       ]
+       HwfCall'
+     ]]
+    ]; subst;
+  destruct Cfg2 as [S2 TD2 Ps2 gl2 fs2];
+  destruct St2 as [ECs2 M2];
+  simpl in Hsim;
+  destruct Hsim as [EQ1 [Hpsim [Hstksim [EQ2 [EQ3 Hmsim]]]]]; subst;
+  destruct ECs2 as [|[F2 B2 cs2 tmn2 lc2 als2] ECs2]; tinv Hstksim;
+  destruct Hstksim as [Hecsim Hstksim];
+  destruct ECs2 as [|[F3 B3 cs3 tmn3 lc3 als3] ECs2]; tinv Hstksim;
+  destruct Hstksim as [Hecsim' Hstksim];
+  unfold EC_simulation in Hecsim;
+  destruct Hecsim as
+      [Hfsim2 [Heq1 [Halsim2 [Hbsim2
+        [Heq3 [Heq4 [Hlcsim2 Hcssim2]]]]]]]; subst;
+  destruct Hecsim' as
+      [Hfsim2' [Heq1' [Halsim2' [Hbsim2'
+        [Heq3' [Heq4' [Hlcsim2' Hcssim2']]]]]]]; subst;
+  apply RemoveSim.cmds_simulation_nil_inv in Hcssim2; subst;
+  wfCall_inv;
+  match goal with 
+  | _: block_simulation _ ?F _ _ |- _ =>
+    assert (HwfF: wf_fdef S (module_intro los nts Ps) F) by
+      eauto 2 using wf_system__wf_fdef;
+    assert (HuniqF: uniqFdef F) by eauto 2 using wf_system__uniqFdef
+  end
+end.
+
 Lemma die_is_sim : forall diinfo Cfg1 St1 Cfg2 St2
   (Hwfpp: OpsemPP.wf_State Cfg1 St1) (Hwfcfg: OpsemPP.wf_Config Cfg1)
   (Hsim: State_simulation diinfo Cfg1 St1 Cfg2 St2),
@@ -741,7 +737,6 @@ Focus.
     eapply returnUpdateLocals_reg_simulation with (lc:=lc);
       eauto 1.
       value_doesnt_use_did_tac.
-
 Unfocus.
 
 SCase "sReturnVoid".
@@ -809,10 +804,8 @@ SCase "sCall".
     apply RemoveSim.fdef_simulation_inv in Hfsim1.
     destruct Hfsim1 as [Hfhsim1 Hbssim1].
     inv Hfhsim1.
-    eapply reg_simulation__initLocals; try solve [
-      eauto 2 |
-      eapply conditional_used_in_fdef__used_in_params; destruct diinfo; eauto 1
-    ].
+    eapply reg_simulation__initLocals; eauto 2;
+      eapply conditional_runused_in_fdef__used_in_params; destruct diinfo; eauto 1.
 
   SSCase "sExCall".
 
@@ -860,7 +853,7 @@ SCase "sExCall".
     inv_mfalse; symmetry_ctx.
     erewrite reg_simulation__params2GVs in H2; eauto.
       uniq_result. auto.
-      eapply conditional_used_in_fdef__used_in_params; destruct diinfo; eauto 1.
+      eapply conditional_runused_in_fdef__used_in_params; destruct diinfo; eauto 1.
   subst.
   uniq_result.
   repeat_solve.
